（IⅡ）解法1：由（I）知， $\angle A^{\prime}O C=120^{\circ}\ldots\ldots\phantom{6}6$ 分如图建系 $O-x y z$ ， $B(1,\ 0,\ 0)$ ，设 $O C=b,O A^{\prime}=a$ ，则 $C(0,\,b,\,0)$ ， $A^{\prime}(0,\ -\frac{1}{2}a,\ \frac{\sqrt{3}}{2}a)$  $\overrightarrow{B C}=(-1,\ b,\ 0)\cdots\cdots=\cdots8$ 分平面 $A^{\prime}D B$ 的法向量为 $\vec{n}=\left(0,\sqrt{3},1\right)\enspace\enspace\mathrm{--}\enspace\enspace\mathrm{--}\enspace\enspace\mathrm{10}$ 分 $\sin45^{\circ}=\left|\cos\left\langle{\vec{n}},{\overrightarrow{B C}}\right\rangle\right|=\left|{\frac{{\vec{n}}\cdot{\overrightarrow{B C}}}{\left|{\vec{n}}\right|\left|{\overrightarrow{B C}}\right|}}\right|\cdots\cdots\cdots-11$  分解得 $\rangle=\sqrt{2}\ ,\ \ B C=\sqrt{3}\ \ \cdots\cdots-12$ 分解法2：由（I）知， $\angle A^{\prime}O C=120^{\circ}\ldots\ldots\phantom{6}6$ 分过 $C$ 作 $C H\bot A^{\prime}O$ ， $B D\perp$ 平面 $A^{\prime}O C$ ， $:B D\perp C H$ ， $C H\bot A^{\prime}O$ ， $C H\perp$ 平面 $A^{\prime}B D$  $\angle C B H$ 就是 $B C$ 与平面 $\Delta A^{\prime}B D$ 所成角--9分设  $C O=x$  ，则  $C H={\frac{\sqrt{3}}{2}}x$  ，  $C B=\sqrt{2}C H=\frac{\sqrt{6}}{2}\,x\;,$  H  $C B={\sqrt{O B^{2}+O C^{2}}}={\sqrt{1+x^{2}}}$ ，则 ${\frac{\sqrt{6}}{2}}x={\sqrt{1+x^{2}}}$ 解得 $x=\sqrt{2}\ ,\ \ B C=\sqrt{3}\ \cdots\cdots-12$ 分  

21.解：  

（I）联立方程组 $\left\{{\begin{array}{l}{y=k x+1}\\ {x^{2}-4y^{2}=4}\end{array}}\right.$ 消 $y$ 得： $\left(1\!-\!4k^{2}\right)\!x^{2}-8k x-8\!=\!0$ -------2分 $\left\{\begin{array}{l l}{\displaystyle1-4k^{2}\neq0}\\ {\Delta=32-64k^{2}>0}\end{array}\right.$ 解得 $-{\frac{\sqrt{2}}{2}}<k<{\frac{\sqrt{2}}{2}}$ 且 $k\neq\pm\frac{1}{2}$ --5分 $k\neq\pm\frac{1}{2}$ 得4分)  

（ⅡI）设 $M$  $N$ 坐标分别为 $\left({{x}_{1}},{{y}_{1}}\right),\left({{x}_{2}},{{y}_{2}}\right)$ ， $A(-2,0)$ ，由(1)知 $\left\{{\begin{array}{l}{\displaystyle x_{1}+x_{2}={\frac{8k}{1-4k^{2}}}}\\ {\displaystyle x_{1}\cdot x_{2}={\frac{-8}{1-4k^{2}}}}\end{array}}\right.$ -6分直线 $M A$ 的方程为 $y=\frac{y_{1}}{x_{1}+2}\big(x+2\big)$ ，令 $\chi=0$ 可得点 $P$ 坐标为 $\left(0,{\frac{2y_{1}}{x_{1}+2}}\right)$ 同理点 $\mathcal{Q}$ 坐标为 $\left(0,{\frac{2y_{2}}{x_{2}+2}}\right)$ -8分 $\left|P Q\right|\!=\!1\!\Rightarrow\!\left|\!\frac{y_{1}}{x_{1}+2}\!-\!\frac{y_{2}}{x_{2}+2}\!\right|\!=\!\frac{1}{2}\!\Rightarrow\!\left|\!\frac{\left(x_{1}-x_{2}\right)\!\left(1-2k\right)}{\left(x_{1}+2\right)\!\left(x_{2}+2\right)}\!\right|\!=\!\frac{1}{2}$   $\left|4{\sqrt{2}}{\sqrt{1-2k^{2}}}\left(1-2k\right)\right|=2\left(2k-1\right)^{2}\cdots\cdots\cdots-10~;$  个  