19. 解: (1) 取 \( {EF} \) 的中点 \( G \) ,连接 \( {DG},{CG} \)

\( \because \) 四边形 \( {AD}{E}_{1}{F}_{1} \) 和 \( {BC}{E}_{2}{F}_{2} \) 都是菱形, \( \angle D{E}_{1}{F}_{1} = \angle C{E}_{2}{F}_{2} = {60}^{ \circ  } \)

![01954211-7bb3-7860-b0e8-7b703eb09aad_0_864_237_313_224_0.jpg](images/01954211-7bb3-7860-b0e8-7b703eb09aad_0_864_237_313_224_0.jpg)

\( \therefore {DG} \bot  {EF} \)

又 \( {BC} = 2 \)

\( \therefore {DG} = {CG} = \sqrt{3} \) 2

又 \( {CD} = {AB} = \sqrt{6} \)

即有 \( D{G}^{2} + C{G}^{2} = C{D}^{2},{DG} \bot  {CG} \) 3

又 \( {CG} \cap  {EF} = G,{CG},{EF} \subset \) 平面 \( {BCEF} \)

\( \therefore {DG} \bot \) 平面 \( {BCEF} \) 5

又 \( {DG} \subset \) 平面 \( {AFED} \)

\( \therefore \) 平面 \( {AFED} \bot \) 平面 \( {BCEF} \) 6

(2)连接 \( {DF},{DB} \)

由 (1) 知 \( {DG} \bot \) 平面 \( {BCEF} \) ,同理 \( {CG} \bot \) 平面 \( {AFED} \) 7

且 \( {S}_{\text{菱形 BCEF }} = 2 \times  \sqrt{3} = 2\sqrt{3},{S}_{\bigtriangleup {ADF}} = \frac{1}{2} \times  2 \times  \sqrt{3} = \sqrt{3} \) - 9

\( V = {V}_{D - {BCEF}} + {V}_{D - {ABF}} = {V}_{D - {BCEF}} + {V}_{B - {ADF}} = \frac{1}{3}{S}_{\text{菱形BCEF }} \cdot  {DG} + \frac{1}{3}{S}_{\Delta ADF} \cdot  {CG} \)

\( = \frac{1}{3} \times  2\sqrt{3} \times  \sqrt{3} + \frac{1}{3} \times  \sqrt{3} \times  \sqrt{3} \) 12

\( = 3 \)

20.解: (1) \( {f}^{\prime }\left( x\right)  = \frac{-m{x}^{2} + 2\left( {m - 1}\right) x + 4}{{e}^{x}} = \frac{-\left( {{mx} + 2}\right) \left( {x - 2}\right) }{{e}^{x}}\left( {m > 0}\right) \)

令 \( {f}^{\prime }\left( x\right)  = 0 \) ,解得 \( x =  - \frac{2}{m} \) 或 \( x = 2 \) ,且 \( - \frac{2}{m} < 2 \) - 2

当 \( x \in  \left( {-\infty , - \frac{2}{m}}\right\rbrack \) 时, \( {f}^{\prime }\left( x\right)  \leq  0 \) ,当 \( x \in  \left( {-\frac{2}{m},2}\right) \) 时, \( {f}^{\prime }\left( x\right)  > 0 \) ,

当 \( x \in  \lbrack 2, + \infty ) \) 时, \( {f}^{\prime }\left( x\right)  \leq  0 \) 4

即 \( f\left( x\right) \) 的单调增区间为 \( \left( {-\frac{2}{m},2}\right) \) ,单调减区间为 \( \left( {-\infty , - \frac{2}{m}}\right\rbrack  ,\lbrack 2, + \infty ) \) 5

(2)由(1)知,当 \( m > 0, x \in  \left\lbrack  {1,2}\right\rbrack \) 时, \( {f}^{\prime }\left( x\right)  > 0 \) 恒成立 6 所以 \( f\left( x\right) \) 在 \( \left\lbrack  {1,2}\right\rbrack \) 上为增函数, 即 \( f{\left( x\right) }_{\max } = f\left( 2\right)  = \frac{{4m} + 2}{{e}^{2}}, f{\left( x\right) }_{\min } = f\left( 1\right)  = \frac{m}{e} \) - 8

\( f\left( {x}_{1}\right)  - f\left( {x}_{2}\right) \) 的最大值为 \( g\left( m\right)  = f{\left( x\right) }_{\max } - f{\left( x\right) }_{\min } = \frac{\left( {4 - e}\right) m + 2}{{e}^{2}} \) - 9

\( \because \frac{4}{{e}^{2}} \geq  \left\lbrack  {f\left( {x}_{1}\right)  - f\left( {x}_{2}\right) }\right\rbrack \) 恒成立 10

\( \therefore \frac{4}{{e}^{2}} \geq  \frac{\left( {4 - e}\right) m + 2}{{e}^{2}} \) ,

即 \( m \leq  \frac{2}{4 - e} \) 11

又 \( m > 0\;\therefore m \in  \left( {0,\frac{2}{4 - e}}\right\rbrack \)

故 \( m \) 的取值范围 \( \left( {0,\frac{2}{4 - e}}\right\rbrack \) 12

21.解: (1) \( \because e = \frac{c}{a} = \frac{\sqrt{2}}{2},\;\therefore {c}^{2} = \frac{1}{2}{a}^{2},\;\therefore {b}^{2} = {a}^{2} - {c}^{2} = \frac{1}{2}{a}^{2} \) . - 2

\( \because \) 椭圆的中心 \( O \) 到直线 \( x + y - {2b} = 0 \) 的距离为 \( 5\sqrt{2} \) ,

\( \therefore \frac{\left| -2b\right| }{\sqrt{2}} = 5\sqrt{2},\therefore b = 5\therefore {b}^{2} = {25},{a}^{2} = 2{b}^{2} = {50} \) .

\( \therefore \) 椭圆 \( C \) 的方程为 \( \frac{{x}^{2}}{50} + \frac{{y}^{2}}{25} = 1 \) .

(2)由(1)可知 \( F\left( {5,0}\right) \) ,由题可知直线 \( {AB} \) 的方程为 \( y = \sqrt{2}\left( {x - 5}\right) \) ,与椭圆 \( C \)

的方程联立 \( \left\{  \begin{array}{l} y = \sqrt{2}\left( {x - 5}\right) \\  \frac{{x}^{2}}{50} + \frac{{y}^{2}}{25} = 1 \end{array}\right. \) ,消去 \( y \) 得 \( {x}^{2} - {8x} + {10} = 0 \)

设 \( A\left( {{x}_{1},{y}_{1}}\right) , B\left( {{x}_{2},{y}_{2}}\right) \) ,则有 \( {x}_{1} + {x}_{2} = 8,{x}_{1}{x}_{2} = {10} \) . 6

设 \( Q\left( {x, y}\right) \) ,由 \( \overrightarrow{OQ} = \lambda \overrightarrow{OA} + \mu \overrightarrow{OB} \) 得 \( \left( {x, y}\right)  = \lambda \left( {{x}_{1},{y}_{1}}\right)  + \mu \left( {{x}_{2},{y}_{2}}\right)  = \left( {\lambda {x}_{1} + \mu {x}_{2},\lambda {y}_{1} + \mu {y}_{2}}\right) \) , \( \therefore \left\{  \begin{array}{l} x = \lambda {x}_{1} + \mu {x}_{2} \\  y = \lambda {y}_{1} + \mu {y}_{2} \end{array}\right. \) - 7