（II）解法 1：由（I）知， $\angle A^{\prime} O C=120^{\circ} \cdots \cdots \cdots \cdots \cdot 6$ 分
如图建系 $O-x y z, B(1,0,0)$, 设 $O C=b, O A^{\prime}=a$, 则 $C(0, b, 0), A^{\prime}\left(0,-\frac{1}{2} a, \frac{\sqrt{3}}{2} a\right)$
$\overline{B C}=(-1, b, 0) \cdots \cdots \cdots \cdots-8$ 分
平面 $A^{\prime} D B$ 的法向量为 $\vec{n}=(0, \sqrt{3}, 1) \cdots \cdots \cdots \cdots-10$ 分
$\sin 45^{\circ}=|\cos \langle\vec{n}, \overline{B C}\rangle|=\left|\frac{\vec{n} \cdot \overline{B C}}{|\vec{n}| \mid B C}\right| \cdots \cdots \cdots \cdots-11$ 分
解得 $b=\sqrt{2}, B C=\sqrt{3} \cdots \cdots \cdots \cdots-12$ 分
解法 2：由（I）知， $\angle A^{\prime} O C=120^{\circ} \cdots \cdots \cdots \cdot 6$ 分
过 $C$ 作 $C H \perp A^{\prime} O, B D \perp$ 平面 $A^{\prime} O C$,
$\therefore B D \perp C H, C H \perp A^{\prime} O, C H \perp$ 平面 $A^{\prime} B D$
$\angle C B H$ 就是 $B C$ 与平面 $\Delta A^{\prime} B D$ 所成角 $\cdots \cdots \cdot 9$ 分
设 $C O=x$, 则 $C H=\frac{\sqrt{3}}{2} x, C B=\sqrt{2} C H=\frac{\sqrt{6}}{2} x$,
![img-0.jpeg](img-0.jpeg)
$C B=\sqrt{O B^{2}+O C^{2}}=\sqrt{1+x^{2}} ，$ 则 $\frac{\sqrt{6}}{2} x=\sqrt{1+x^{2}}$
解得 $x=\sqrt{2}, B C=\sqrt{3} \cdots \cdots \cdots \cdots-12$ 分
21. 解:
（I）联立方程组 $\left\{\begin{array}{l}y=k x+1 \\ x^{2}-4 y^{2}=4\end{array}\right.$ 消 $y$ 得: $\left(1-4 k^{2}\right) x^{2}-8 k x-8=0 \quad-\cdots \cdots \cdot 2$ 分
$\left\{\begin{array}{l}1-4 k^{2} \neq 0 \\ \Delta=32-64 k^{2}>0\end{array}\right.$ 解得 $-\frac{\sqrt{2}}{2}<k<\frac{\sqrt{2}}{2}$ 且 $k \neq \pm \frac{1}{2} \cdot \cdots \cdots \cdot 5$ 分
（漏 $k \neq \pm \frac{1}{2}$ 得 4 分）
（II）设 $M, N$ 坐标分别为 $\left(x_{1}, y_{1}\right),\left(x_{2}, y_{2}\right), A(-2,0)$ ，由（I）知
$\left\{\begin{array}{l}x_{1}+x_{2}=\frac{8 k}{1-4 k^{2}} \\ x_{1} \cdot x_{2}=\frac{-8}{1-4 k^{2}}\end{array}\right.$

直线 $M A$ 的方程为 $y=\frac{y_{1}}{x_{1}+2}(x+2)$, 令 $x=0$ 可得点 $P$ 坐标为 $\left(0, \frac{2 y_{1}}{x_{1}+2}\right)$
同理点 $Q$ 坐标为 $\left(0, \frac{2 y_{2}}{x_{2}+2}\right) \cdots \cdots \cdots \cdot-8$ 分
$|P Q|=1 \Rightarrow\left|\frac{y_{1}}{x_{1}+2}-\frac{y_{2}}{x_{2}+2}\right|=\frac{1}{2} \Rightarrow\left|\frac{\left(x_{1}-x_{2}\right)(1-2 k)}{\left(x_{1}+2\right)\left(x_{2}+2\right)}\right|=\frac{1}{2}$
$\left|4 \sqrt{2} \sqrt{1-2 k^{2}}(1-2 k)\right|=2(2 k-1)^{2} \cdots \cdots \cdots-10$ 分