19. 解:(1) 取 \( EF \) 的中点 \( G \), 连接 \( DG \), \( CG \)
\( \therefore \) 四边形 \( ADEF_1 \) 和 \( BCE_2F_2 \) 都是菱形, \( \angle DEF_1 = \angle CE_2F_2 = 60^\circ \)
\( \therefore DG \perp EF \)
又 \( BC = 2 \)
\( \therefore DG = CG = \sqrt{3} \)
又 \( CD = AB = \sqrt{6} \)
即有 \( DG^2 + CG^2 = CD^2 \), \( DG \perp CG \)
又 \( CG \cap EF = G \), \( CG, EF \subset 平面 BCEF \)
\( \therefore DG \perp 平面 BCEF \)
又 \( DG \subset 平面 AFED \)
\( \therefore 平面 AFED \perp 平面 BCEF \)
(2) 连接 \( DF \), \( DB \)
由(1)知 \( DG \perp 平面 BCEF \), 同理 \( CG \perp 平面 AFED \)
且 \( S_{菱形 BCEF} = 2 \times \sqrt{3} = 2\sqrt{3} \), \( S_{\triangle ADF} = \frac{1}{2} \times 2 \times \sqrt{3} = \sqrt{3} \)

\( V = V_{D-BCEF} + V_{D-ABF} = V_{D-BCEF} + V_{B-ADF} = \frac{1}{3} S_{菱形 BCEF} \cdot DG + \frac{1}{3} S_{\triangle ADF} \cdot CG \)
\( = \frac{1}{3} \times 2\sqrt{3} \times \sqrt{3} + \frac{1}{3} \times \sqrt{3} \times \sqrt{3} \)
\( = 3 \)
所以 \( f(x) \) 在 \( [1,2] \) 上为增函数,
即 \( f(x)_{max} = f(2) = \frac{4m+2}{e^2} \), \( f(x)_{min} = f(1) = \frac{m}{e} \)
\( f(x_1) - f(x_2) \) 的最大值为 \( g(m) = f(x)_{max} - f(x)_{min} = \frac{(4-e)m+2}{e^2} \)
\( \therefore \frac{4}{e^2} \ge [f(x_1) - f(x_2)] \) 恒成立
\( \therefore \frac{4}{e^2} \ge \frac{(4-e)m+2}{e^2} \)
即 \( m \le \frac{2}{4-e} \)
又 \( m > 0 \)   \( \therefore m \in (0, \frac{2}{4-e}] \)

故 \( m \) 的取值范围 \( (0, \frac{2}{4-e}] \)
21. 解: (1) \( \because e = \frac{c}{a} = \frac{\sqrt{2}}{2}, \therefore c^2 = \frac{1}{2} a^2, \therefore b^2 = a^2 - c^2 = \frac{1}{2} a^2 \)
\( \therefore \) 椭圆的中心 \( O \) 到直线 \( x + y - 2b = 0 \) 的距离为 \( 5\sqrt{2} \),
\( \therefore \frac{|-2b|}{\sqrt{2}} = 5\sqrt{2}, \therefore b = 5 \)   \( \therefore b^2 = 25, a^2 = 2b^2 = 50 \)
\( \therefore \) 椭圆 \( C \) 的方程为 \( \frac{x^2}{50} + \frac{y^2}{25} = 1 \)
(2) 由(1) 可知 \( F(5,0) \), 由题可知直线 \( AB \) 的方程为 \( y = \sqrt{2}(x - 5) \), 与椭圆 \( C \)
\( \begin{cases} y = \sqrt{2}(x - 5) \\ \frac{x^2}{50} + \frac{y^2}{25} = 1 \end{cases} \), 消去 \( y \) 得 \( x^2 - 8x + 10 = 0 \)
设 \( A(x_1, y_1), B(x_2, y_2) \), 则有 \( x_1 + x_2 = 8, x_1x_2 = 10 \)
设 \( Q(x, y) \), 由 \( \overrightarrow{OQ} = \lambda \overrightarrow{OA} + \mu \overrightarrow{OB} \) 得 \( (x, y) = \lambda (x_1, y_1) + \mu (x_2, y_2) = (\lambda x_1 + \mu x_2, \lambda y_1 + \mu y_2) \),
\( \begin{cases} x = \lambda x_1 + \mu x_2 \\ y = \lambda y_1 + \mu y_2 \end{cases} \)

20. 解: (1) \( f'(x) = \frac{-mx^2 + 2(m - 1)x + 4}{e^x} = \frac{-(mx + 2)(x - 2)}{e^x} \)  \( (m > 0) \)
令 \( f'(x) = 0 \), 解得 \( x = -\frac{2}{m} \) 或 \( x = 2 \), 且 \( -\frac{2}{m} < 2 \)
当 \( x \in (-\infty, -\frac{2}{m}] \) 时, \( f'(x) \le 0 \), 当 \( x \in (-\frac{2}{m}, 2) \) 时, \( f'(x) > 0 \)
当 \( x \in [2, +\infty) \) 时, \( f'(x) \le 0 \)
即 \( f(x) \) 的单调增区间为 \( (-\frac{2}{m}, 2) \), 单调减区间为 \( (-\infty, -\frac{2}{m}], [2, +\infty) \)
(2) 由(1)知, 当 \( m > 0, x \in [1,2] \) 时, \( f'(x) > 0 \) 恒成立
