{"primary_language":"zh","is_rotation_valid":true,"rotation_correction":0,"is_table":false,"is_diagram":false,"natural_text":"（II）解法 1：由（I）知，$$\\angle A'OC = 120^\\circ$$ 6 分\n\n如图建立系 $$O \\cdots$$, $$B(1, 0, 0)$$，设 $$OC = b$$, $$OA' = a$$，则 $$C(0, b, 0)$$, $$A'(0, -\\frac{1}{2}a, \\frac{\\sqrt{3}}{2}a)$$\n$$\\overrightarrow{BC} = (-1, b, 0)$$ 8 分\n\n平面 $$A'DB$$ 的法向量为 $$\\overrightarrow{n} = (0, \\sqrt{3}, 1)$$ 10 分\n\n$$\\sin 45^\\circ = \\left| \\cos \\left( \\overrightarrow{n}, \\overrightarrow{BC} \\right) \\right| = \\left| \\frac{\\overrightarrow{n} \\cdot \\overrightarrow{BC}}{||\\overrightarrow{n}|| ||\\overrightarrow{BC}||} \\right|$$ 11 分\n\n解得 $$b = \\sqrt{2}, \\quad BC = \\sqrt{3}$$ 12 分\n\n解法 2：由（I）知，$$\\angle A'OC = 120^\\circ$$ 6 分\n\n过 $$C$$ 作 $$CH \\perp A'O$$, $$BD \\perp$$ 平面 $$A'OC$$,\n$$\\therefore BD \\perp CH$$, $$CH \\perp A'O$$, $$CH \\perp$$ 平面 $$A'BD$$\n$$\\angle CBH$$ 就是 $$BC$$ 与平面 $$A'B$$ 所成角 9 分\n\n设 $$CO = x$$，则 $$CH = \\frac{\\sqrt{3}}{2}x$$, $$CB = \\sqrt{2}CH = \\frac{\\sqrt{6}}{2}x$$，\n$$CB = \\sqrt{OB^2 + OC^2} = \\sqrt{1 + x^2}$$，则 $$\\frac{\\sqrt{6}}{2}x = \\sqrt{1 + x^2}$$\n\n得 $$x = \\sqrt{2}, \\quad BC = \\sqrt{3}$$ 12 分\n\n21. 解:\n\n(I) 联立方程组\n$$\\begin{cases} y = kx + 1 \\\\ x^2 - 4y^2 = 4 \\end{cases}$$ 消 $$y$$ 得：$$\\left(1 - 4k^2\\right)x^2 - 8kx - 8 = 0$$ 2 分\n\n$$\\begin{cases} 1 - 4k^2 \\neq 0 \\\\ \\Delta = 32 - 64k^2 > 0 \\end{cases}$$ 解得：$$-\\frac{\\sqrt{2}}{2} < k < \\frac{\\sqrt{2}}{2}$$ 且 $$k \\neq \\pm \\frac{1}{2}$$ 5 分\n\n(l) $$x_1 + x_2 = \\frac{8k}{1 - 4k^2}$$ 6 分\n\n$$x_1 \\cdot x_2 = -8$$ 6 分\n\n(I) 设 $$M, N$$ 坐标分别为 $$(x_1, y_1), (x_2, y_2), A(-2, 0)$$，由 (I) 知\n\n$$\\begin{cases} x_1 + x_2 = \\frac{8k}{1 - 4k^2} \\\\ x_1 \\cdot x_2 = -8 \\end{cases}$$ 6 分\n\n直线 $$MA$$ 的方程为 $$y = \\frac{y_1}{x_1 + 2}(x + 2)$$，令 $$x = 0$$ 可得点 $$P$$ 坐标为 $$(0, \\frac{2y_1}{x_1 + 2})$$\n\n同理由 $$Q$$ 坐标为 $$(0, \\frac{2y_2}{x_2 + 2})$$ 8 分\n\n$$|PQ| = 1 \\Rightarrow \\left| \\frac{y_1}{x_1 + 2} - \\frac{y_2}{x_2 + 2} \\right| = \\frac{1}{2} \\Rightarrow \\left| \\frac{(x_1 - x_2)(1 - 2k)}{(x_1 + 2)(x_2 + 2)} \\right| = \\frac{1}{2}$$\n\n$$4\\sqrt{2}\\sqrt{1 - 2k^2} (1 - 2k) = 2(2k - 1)^2$$ 10 分"}