```markdown
\[
\begin{aligned}
\because \tan 2 \alpha = \frac{2 \tan \alpha}{1 - \tan^2 \alpha} = \tan \beta, \\
\therefore \frac{2 \tan \alpha}{1 - \tan^2 \alpha} = -\frac{1}{\tan \alpha}, \\
\therefore \tan^3 \alpha + 2 \tan \alpha = 0, \\
\therefore \tan \alpha = 0 \text{ æˆ– } \tan \alpha = \pm \sqrt{2}.
\end{aligned}
\]

\[
\begin{aligned}
\because \tan 2 \alpha = \frac{1}{\tan \alpha} = \tan \beta, \\
\therefore \tan \alpha = \frac{1}{\tan \alpha}, \\
\therefore \tan^2 \alpha = 1, \\
\therefore \tan \alpha = \pm 1.
\end{aligned}
\]

\[
\begin{aligned}
\because \tan 3 \alpha = \frac{\tan 2 \alpha + \tan \alpha}{1 - \tan 2 \alpha \tan \alpha} = \tan \beta, \\
\therefore \frac{\tan 2 \alpha + \tan \alpha}{1 - \tan 3 \alpha \tan \alpha} = -\frac{1}{\tan \alpha}, \\
\therefore (\tan 2 \alpha + \tan \alpha)(1 - \tan 2 \alpha \tan \alpha) = -1, \\
\therefore \tan 2 \alpha \tan \alpha - \tan^2 \alpha - \tan 2 \alpha = -1, \\
\therefore \tan 2 \alpha (\tan \alpha - 1) - \tan^2 \alpha - 1 = 0, \\
\therefore \tan 2 \alpha (\tan \alpha - 1) = \tan^2 \alpha + 1, \\
\therefore \tan 2 \alpha (\tan \alpha - 1)^2 = \tan^2 \alpha + 1, \\
\therefore \tan 2\alpha = \frac{\tan^2 \alpha + 1}{(\tan \alpha - 1)^2}, \\
\therefore \tan 2 \alpha = \frac{\tan^2 \alpha + 1}{\tan^2 \alpha - 2 \tan \alpha + 1}, \\
\therefore \tan 2 \alpha = \frac{\tan^2 \beta + 1}{\tan^2 \beta - 2 \tan \beta + 1}, \\
\therefore \tan 2 \alpha = \frac{\tan \beta - 1}{\tan \beta + 1}, \\
\therefore \tan 2 \alpha = \tan (\beta - \frac{\pi}{4}), \\
\therefore 2 \alpha = \beta - \frac{\pi}{4} + k \pi, \\
\therefore \alpha = \frac{\beta}{2} - \frac{\pi}{8} + \frac{k \pi}{2}.
\end{aligned}
\]

\[
\begin{aligned}
\because \sin 2 \alpha = \frac{2 \sin \alpha \cos \alpha}{\sin^2 \alpha + \cos^2 \alpha} = \sin \beta, \\
\therefore \frac{2 \sin \alpha \cos \alpha}{\sin^2 \alpha \cos^2 \alpha} = \sin \beta, \\
\therefore \frac{\sin \alpha \cos \alpha}{\sin^2 \alpha \cos^2 \beta} = \frac{1}{2} \sin \beta, \\
\therefore \sin \alpha \cos \alpha = \frac{1}{2} \sin \beta \sin^2 \alpha \cos^2 \beta, \\
\therefore \sin \alpha \cos \alpha = \frac{3}{4} \sin \beta \sin^2 \alpha \cos^2 \beta, \\
1 - \cos^2 \alpha = \frac{3}{4} \sin \beta \sin^2 \beta \cos^2 \beta, \\
\therefore \cos^2 \alpha = 1 - \frac{3}{4} \sin \beta \sin^2 \beta \cos \beta, \\
\therefore \cos^2 \alpha = \frac{1}{4} \sin \beta \sin^2 \beta \cos \beta, \\
1 - \cos^2 \alpha = \frac{1}{4} \sin \beta \cos \beta, \\
\therefore \cos^2 \alpha = \cos^2 \beta, \\
\therefore \cos \alpha = \cos \beta, \\
\therefore \alpha = \beta + k \pi.
\end{aligned}
\]

\[
\begin{aligned}
\because \sin 3 \alpha = \frac{3 \sin \alpha - 4 \sin^3 \alpha}{\sin^2 \alpha + \cos^2 \alpha} = \cos \beta, \\
\therefore \frac{3 \sin \alpha - 4 \sin^3 \alpha}{\cos^2 \alpha + \sin^2 \alpha} = \cos \beta, \\
\therefore \frac{3}{\cos^2 \alpha + \sin^2 \alpha} - \frac{4 \sin^3 \alpha}{\cos^2 \alpha + \sin^2} = \cos \beta, \\
\therefore \frac{3}{\cos^3 \alpha + \sin^3 \alpha} - \frac{4 \sin^3 \alpha}{\cos^3 \alpha + \sin^3 \alpha} = \cos \beta, \\
\therefore \frac{3}{\sin^3 \alpha + \cos^3 \alpha} - \frac{4 \sin^3 \alpha}{\sin^3 \alpha + \cos^3 \alpha} = \cos \beta, \\
\therefore \frac{3 \cos^3 \alpha - 4 \sin^3 \alpha}{\sin^3 \alpha + \cos^3} = \cos \beta, \\
\therefore \frac{3 \cos^3}{\sin^3 \alpha + \cos^3 \alpha} - \frac{\sin^3 \alpha}{\sin^3 \alpha + \cos^3 \alpha}
\end{aligned}
```