```markdown
\[
\begin{aligned}
&\because \left[\left(2 a+\frac{3 \sqrt{2}}{b}\right)^{2}+\left(2 b+\frac{6 \sqrt{2}}{b}-\frac{3 \sqrt{2}}{b}\right)^{2}\right]-\left(\frac{6 \sqrt{2}}{b}\right)^{2} \\
&=\left(2 a+\frac{3 \sqrt{2}}{b}\right)^{3}+\left(2 b+\frac{6 \sqrt{2}}{b}-\left(\frac{6 \sqrt{2}}{b}\right)^{2}\right)^{2} \\
&\therefore a b=\sqrt{3} \\
&\because B\left(3,2 \sqrt{3}\right), D\left(2,3 \sqrt{6}\right), \\
&\therefore \text{直线 } O B \text{的解析式为 } y=2 \sqrt{2} x, \text{直线 } D F \text{的解析式为 } y=2 \sqrt{2} x-3 \sqrt{6}, \text{当 } y=0 \text{时}, 2 \sqrt{2} x-3 \sqrt{6}=0, \\
&\therefore x=\frac{3 \sqrt{3}}{2}, \\
&\therefore F\left(\frac{3 \sqrt{3}}{2}, 0\right), \\
&\therefore O E=\sqrt{3}, O F=\frac{3 \sqrt{3}}{2}, \\
&\therefore E F=O F-O E=\frac{3 \sqrt{3}}{2}-\sqrt{3}=\frac{\sqrt{3}}{2}, \\
&\therefore \frac{E F}{O E}=\frac{1}{2}, \\
&\therefore \text{故答案为: } \frac{1}{2}\left(\frac{3 \sqrt{3}}{2}, 0\right)
\end{aligned}
\]

\[
\begin{aligned}
&\because \left[\left(2 a+\frac{\sqrt{2}}{b}\right)^{2}+\left(2 b+\frac{\sqrt{2}}{b}-\frac{\sqrt{2}}{b}\right)^{2}\right]-\left(\frac{\sqrt{2}}{b}\right)^{2} \\
&=\left(2 a-\frac{\sqrt{2}}{b}\right)^{2}+\left(2 b-\frac{\sqrt{2}}{b}-\left(\frac{\sqrt{2}}{b}\right)^{2}\right)^{2} \\
&=\left(2 a-\frac{\sqrt{2}+1}{b}\right)^{2}+\left(2 b-\frac{\sqrt{2}+1}{b}-\left(\frac{\sqrt{2}+1}{b}\right)^{2}\right)^{2} \\
&=\left(2 a+\frac{\sqrt{2}+1}{b}\right)^{2}+\left(3 b-\frac{\sqrt{2}+1}{b}-\left(\frac{\sqrt[3]{2}+1}{b}\right)^{2}\right)^{2} \\
&\therefore a b=1 \\
&\because B\left(3,2 \sqrt{3}\right), D(2,3 \sqrt{6}), \\
&\therefore \text{直线 } O B \text{的解析为 } y=2 \sqrt{2} x, \text{直线 } D E \text{的解析式为 } y=2 \sqrt{2} x-6 \sqrt{2}, \text{当 } y=0 \text{时}, 2 \sqrt{3} x-6 \sqrt{2}=0, \\
&\therefore x=3 \sqrt{2}, \\
&\therefore F(3 \sqrt{2}, 0), \\
&\therefore O E=3 \sqrt{2}, O F=3 \sqrt{2}, \\
&\therefore E F=O F-O E=3 \sqrt{2}-3 \sqrt{2}=0, \\
&\therefore \frac{E F}{O E}=\frac{0}{3 \sqrt{2}}=0, \\
&\therefore \text{故答案为: } 0
\end{aligned}
\]

\[
\begin{aligned}
&\because \left(2 a+\frac{\sqrt{2}}{b}\right)^{2}=\left(2 b+\frac{\sqrt{2}}{b}-\frac{\sqrt{3}}{b}\right)^{2} \\
&=\left(2 b+\frac{\sqrt{2}}{b}-\left(\frac{\sqrt{2}}{2}\right)^{2}\right)^{2} \\
&=\left(2 b+\frac{\sqrt{2}+1}{b}\right)^{2}+\left(\frac{\sqrt{2}+1}{b}-\left(\frac{\sqrt{2}}{2}\right)^{2}\left(\frac{\sqrt{2}+1}{b}\right)^{2}\right) \\
&=\left(2 a+\frac{\sqrt{2}+1}{b}\left(\frac{\sqrt{2}+1}{b}\right)^{2}\left(\frac{\sqrt{2}+1}{b}\left(\frac{\sqrt{2}+\sqrt{2}}{b}\right)^{2}\right)^{2} \\
&=0 \\
&\therefore a b=0 \\
&\because B\left(3,2 \sqrt{3}\right), D=2,3 \sqrt{6}, \\
&\therefore \text{直线 } O B \text{的解析 } y=2 \sqrt{2} x, \text{直线 } D E=2 \sqrt{2} x-6 \sqrt{2}, \text{当} y=0 \text{时}, 2 \sqrt{2} x-6 \sqrt{2}=0, \\
&\therefore x=3, \\
&\therefore F(3,0), \\
&\therefore O E=3, O F=3, \\
&\therefore E F=O F-O E=3-3=0, \\
&\therefore \frac{E F}{O E}=\frac{1}{3}, \\
&\therefore \text{故答案为: } \frac{1}{3}
\end{aligned}
\]

\[
\begin{aligned}
&\because \left(\frac{3 \sqrt{2}}{b}\right)^{2}+\left(\frac{6 \sqrt{2}}{b}-\frac{3 \sqrt{2}+1}{b}\right)^{2} \\
&=\left(\frac{3 \sqrt{2}}{b}\right)^{2}+\frac{6 \sqrt{2}}{b}-\left(\frac{3 \sqrt{2}+1}{b}\right)^{2} \\
\end{aligned}
\]

\[
\begin{aligned}
&\because \left[2 a+\frac{3 \sqrt{2}}{b}\right)^{2}=\left(2 b+\frac{6 \sqrt{2}}{b}-\frac{6 \sqrt{2}}{b}\right)^{2} \\
&=\frac{6 \sqrt{2}}{b}-\left(\frac{6 \sqrt[3]{2}}{b}\right)^{2} \\
&=\left(2 a+\frac{\sqrt{2}}{b}\right)^{2} \\
&=\left(3 b+\frac{\sqrt{2}}{b}-\left(\frac{\sqrt{2}+1}{b}\right)^{3}\right)^{2} \\
&=\left(2 a+\frac{\sqrt{2}-1}{b}\right)^{2} \\
&=\left(2 b+\frac{\sqrt{3}}{b}-\left(\frac{\sqrt{2}+1}{b}\right)\right)^{2} \\
&=\left(2 a+\frac{\sqrt{2}-2}{b}\right)^{2} \\
&=\left(2 b+\frac{\sqrt[3]{2}}{b}-\left(\frac{\sqrt{2}+1}{b}\left(\frac{\sqrt{3}}{b}\right)^{2}\right)^{2} \\
&=\left(3 b+\frac{\sqrt{2}-1}{b}-\left(\frac{\sqrt{2}+1}{b}\left(\frac{3 \sqrt{2}}{b}\right)^{2}\right)^{2} \\
\end{aligned}
\]

\[
\begin{array}{l}
\text{解析:} \\
\text{解析:} \\
\text{解析:} \\
\text{故答案为:} \frac{1}{2}\left(\frac{3 \sqrt{3}}{2}\right) \\
\text{故答案为:} 0 \\
\text{故答案为:} \frac{1}{3}
\end{array}
\]

\[
\begin{aligned}
&\because \left(2 a+\left(\frac{3 \sqrt{2}}{b}\right)^{2}\right)+\left(2 b+\left(\frac{6 \sqrt{2}}{b}-\frac{3 \left(\sqrt{2}+1\right)}{b}\right)^{2}\right) \\
&=\left(2 a+\left(\frac{3 \sqrt{2}}{b}\right)\right)^{2}+\left(2 b+\left(\frac{6 \sqrt{2}}{b}-\left(\frac{3 \left(\sqrt{2}+1\right)}{b}\right)\right)^{2} \\
&=\left(2 a+\left(\frac{3 \sqrt{2}}{2}\right)\right)^{2}+\left(2 b+\left(\frac{6}{b}-\left(\frac{3 \left(\sqrt{2}+1\right)^{2}}{b}\right)\right)^{2} \\
&=\left(2 a+\left(3 \sqrt{2}\right)\right)^{2}+\left(2 b+\left(\frac{\sqrt{2}}{b}-\left(\frac{3 \left(\sqrt{2}-1\right)}{b}\right)\right)^{2} \\
&=\left(3 b+\left(\frac{\sqrt{2}}{b}-\left(\frac{3}{b}\right)\right)^{2}+\left(2 a+\left(\frac{\sqrt{2}}{b}-\left(\frac{3}{2}\right)\right)^{2} \\
&=\left(2 a+\left(\frac{\sqrt{2}}{b}-\left(\sqrt{2}-1\right)\right)^{2}+\left(2 b+\left(\frac{\sqrt{3}}{b}-\left(\frac{3}{2}\right)\right)^{2}
\end{aligned}
\]

\[
\begin{aligned}
&\because \frac{3 \sqrt{2}}{b}=\frac{6 \sqrt{2}}{b}-\frac{3 \sqrt{2}-1}{b} \\
&=\left(2 a+\left(\frac{3 \sqrt{2}}{\sqrt{2}}\right)\right)^{2}+\left(2 b+\left(\frac{6 \left(\sqrt{2}+1\right)}{b}-\left(\frac{3 \left(\sqrt{2}+1\left(\sqrt{2}+1\right)}{b}\right)\right)^{3} \\
&=\left(2 a+\left(\frac{3 \sqrt{2}}{-\sqrt{2}}\right)\right)^{2}+\left(2 b+\left(-\frac{6 \left(\sqrt{2}+1\right)}{b}-\frac{3 \left(\sqrt{2}+1\left(\sqrt{2}+\sqrt{2}\right)}{b}\right)\right)^{2} \\
&=\left(2 a-\left(\frac{3 \sqrt{2}}{\sqrt{2}}\right)\right)+\left(2 b-\left(\frac{6 \left(\sqrt{2}+1\right)}{b}+\frac{3 \left(\sqrt{2}+1\left(\sqrt{2}-\sqrt{2}\right)}{b}\right)\right)^{2} \\
&=\frac{3 \sqrt{2}}{b}=\frac{6 \sqrt{2}-3 \sqrt{2}-1}{b} \\
&=\left(2 a+\left(3 \sqrt{2}\right)\left(\frac{3 \sqrt{2}}{b}-\left(\frac{3 \left(\sqrt{3}+1\right)}{b}\right)\right)^{2}+\left(2 b+\left(\frac{\sqrt[3]{2}}{b}-\left(\frac{3 \left(\sqrt{2}+2\right)}{b}\right)\right)^{2} \\
&=\left(2 b+\left(\frac{\sqrt[3]{2}}{b}-\frac{3 \left(\sqrt{2}+2\right)}{b}\right)^{2}+\left(2 a+\left(\frac{\sqrt[3]{2}}{b}-\frac{3 \sqrt{2}}{b}\right)\right)^{2} \\
&=\left(2 b+\left(-\frac{\sqrt[3]{2}}{b}-\frac{3 \left(\sqrt[3]{2}+2\right)}{b}\right)^{2}+\left(2 b+\left(-\frac{\sqrt[3]{2}}{b}-3 \sqrt{2}\right)\right)^{2} \\
&=\left(2 a+\left(-\frac{\sqrt[3]{2}}{b}-\frac{3}{b}\right)\right)^{2}+\left(2 b+\left(-\frac{\sqrt[3]