```markdown
19. 解: (1) 取 EF 的中点 G, 连接 DG, CG
\[
\begin{aligned}
\because & \text{四边形} ADE_1F_1 \text{和} BCE_1F_1 \text{都是菱形,} \angle DE_1F_1 = \angle CE_1F_1 = 60^\circ \\
\therefore & DG \perp EF \quad \quad \quad \quad \quad \quad \quad \quad \quad \quad \text{(1)} \\
& \text{又} BC = 2 \\
\therefore & DG = CG = \sqrt{3} \quad \quad \quad \quad \quad \quad \quad \quad \quad \ \ \text{(2)} \\
& \text{又} CD = AB = \sqrt{6} \\
\therefore & DG^2 + CG^2 = CD^2, \quad DG \perp CG \quad \quad \quad \quad \quad \quad \quad \quad \quad \ 3 \\
& \text{又} CG \cap EF = G, \quad CG, EF \subset \text{平面} BCE_1F_1 \\
\therefore & DG \perp \text{平面} BCE_1F_1 \quad \quad \quad \quad \quad \quad \quad \quad \quad \   5 \\
& \text{又} DG \subset \text{平面} AFE_1D \\
\therefore & \text{平面} AFE_1D \perp \text{平面} BCE_1F_1 \quad \quad 6 \\
\because & \text{平面} AFE_1D \cap \text{平面} BCE_1F_1 = E_1F_1 \\
\therefore & \text{连接} DF_1, \quad DB \quad \quad \quad \quad \quad \quad \quad \quad \quad \    7 \\
\because & DG \perp \text{平面} BCE_1F_1, \quad CG \subset \text{平面} BCE_1F_1 \\
\therefore & CG \perp DG \quad \quad \quad \quad \quad \quad \quad \quad \quad \     8 \\
\therefore & S_{\triangle ADF_1} = \frac{1}{2} \times 2 \times \sqrt{3} \times \sqrt{3} = \sqrt{3} \quad \quad \quad \quad \quad \quad \ \ \text{(9)} \\
\because & V = V_{D-BCF_1} + V_{D-ABF_1} = V_{D-BCF_1} + V_{B-ADF_1} = \frac{1}{3} S_{\triangle ADF_1} \cdot DG + \frac{1}{3} S_{\triangle ADF_1} \cdot CG \\
\therefore & V = \frac{1}{3} \times \sqrt{3} \times \sqrt{3} + \frac{1}{3} \times \sqrt{3} \times \sqrt{2} = \frac{1}{3} \times 2 \times \sqrt{3} \times \sqrt{3} \quad \quad \quad \quad \quad \quad \quad 12 \\
\because & \frac{1}{2} \times 2 \times \sqrt{3} \cdot \sqrt{3} = \frac{1}{3} \times 2 \times \sqrt{3}
\end{aligned}
\]

所以 \( f(x) \) 在 \([2,+\infty)\) 上为增函数,
\[
\begin{aligned}
\because & f(x)_{\max} = f(2) = 2 + \frac{m}{e^2}, \quad f(x)_{\min} = f(0) = \frac{m}{e} \\
\therefore & f(x) - f(x)_{\max} = \frac{m}{e} - \frac{m}{e^2} = \frac{(4-e)m}{e^2} \quad \quad \quad \quad \quad \quad \quad \quad \quad 8 \\
\because & \frac{4}{e^2} \leq f(x) - f(x)_{\min} \text{恒成立} \quad \quad \quad \quad \quad \quad \quad \quad \quad \\
\therefore & \frac{4}{e^2} \leq (4-e)m + 2, \quad \quad \quad \quad \quad \quad \quad \quad \quad \ \
\end{aligned}
\]

即 \( m \leq \frac{2}{4-e} \quad \quad \quad \quad \quad \quad \quad \quad \quad (11) \)

又 \( m > 0 \quad \therefore \quad m \in \left(0, \frac{2}{4-e}\right] \quad \quad \quad \quad \quad \quad \quad \quad \quad \ (12) \)

故 \( m \) 的取值范围为 \(\left(0, \frac{2}{4-e}\right] \quad \quad \ \ \ \ \ \ \ \ \ \ \ \ \ \ \ \ \ \ \ \ (13) \)

且 \( S_{\triangle ACF_1} = 2 \times \sqrt{3} \times 2 \sqrt{3}, \quad S_{\triangle ADF_1} = \frac{1}{2} \times \sqrt{3} \times \sqrt{3} = \sqrt{3}, \quad S_{\triangle ADF_1} = \frac{\sqrt{3}}{3} \quad \quad \quad \quad \quad \quad \quad \quad (14) \)

\[
\begin{aligned}
\because & V = V_{D-BCF_1} + V_{D-ADF_1} = V_{D-BCF_1} + V_{B-ADF} = \frac{1}{3} S_{\triangle ADF_1} \times DG + \frac{1}{3} S_{\triangle ADF_1} \times CG \\
\therefore & V = \frac{1}{3} \times \sqrt[3]{3} \times \sqrt[3]{3} + \frac{1}{3} \times \sqrt[3]{3} \times \frac{\sqrt{3}}{3} = \frac{1}{3} \times 2 \times \sqrt[3]{3} \times \sqrt[3]{3} \quad \quad \quad \quad \quad \quad \quad \quad \ \ \ \ \ \ \ \ \ \ \ \ \ \ \ (15) \\
\because & \frac{1}{2} \times 2 \times \sqrt[3]{3} \times \sqrt[2]{3} = \frac{1}{3} \times 2 \times \sqrt[2]{3}
\end{aligned}
\]

21. 解: (1) \(\because \frac{c}{a} = \frac{\sqrt{2}}{2}, \quad \therefore \frac{c^2}{a^2} = \frac{1}{2}, \quad \therefore b^2 = a^2 - c^2 = \frac{1}{2} a^2 \quad \quad \quad \quad \quad \quad \quad \quad \quad \) (2)

\[
\begin{aligned}
\because & \text{椭圆的中点} O \text{到直线} x = y + 2b = 0 \text{的距离为} \frac{5 \sqrt{2}}{2}, \\
\therefore & \frac{|2b|}{\sqrt{2}} = 5 \sqrt{2}, \quad \therefore b = 5, \quad b^2 = 25, \quad a^2 = 2b^2 = 50. \\
\therefore & \text{椭圆} C \text{的方程为} \frac{x^2}{50} + \frac{y^2}{25} = 1. \quad \quad \quad \quad \quad \quad \quad \quad \quad \ \\
\because & \text{椭圆} C \text{的方程为} \frac{y^2}{25} = 1, \quad \text{由题可知直线} AB \text{的方程为} y = \sqrt{2}(x-5), \quad \text{与椭圆} C \\
\therefore & \text{联立} \begin{cases} y = \sqrt{2}(x-5) \\ \frac{x^2}{50} + \frac{y^2}{25} =1 \end{cases} \quad \quad \quad \quad \quad \quad \quad \quad \quad
\end{aligned}
\]

消去 \( y \) 得 \( x^2 - 8x + 10 = 0 \quad \quad \quad \quad \quad \quad \quad \quad \quad \)

设 \( A(x_1, y_1), \quad B(x_2, y_2) \), 则有 \( x_1 + x_2 = 8, \quad x_1 x_2 = 10 \quad \quad \quad \quad \quad \quad \quad \quad \quad \)
设 \( Q(x, y) \), 由 \( Q(x, y) \) 在椭圆 \( C \) 上, 得 \( \frac{x^2}{50} + \frac{y^2}{25} = \frac{x^2}{50} + \frac{(\sqrt{2}x - 5\sqrt{2})^2}{25} = 1 \quad \quad \quad \quad \quad \quad \quad \quad \quad (7) \)

\[
\begin{aligned}
\therefore & y = \sqrt{2}x + 5\sqrt{2} \\
\because & y = \sqrt{2}x + 5\sqrt{2}
\end{aligned}
\]

20. 解: (1) \( f'(x) = -mx^2 + 2(m-1)x + 4 = -(mx^2 - 2(m-1)x - 4) \quad \quad \quad \quad \quad \quad \quad \quad \quad \ (\text{1}) \)

令 \( f'(x) = 0 \), 解得 \( x = \frac{2}{m} \) 或 \( x = 2 \), 且 \( \frac{2}{m} < 2 \quad \quad \quad \quad \quad \quad \quad \quad \quad (2) \)

当 \( x \in \left(-\infty, \frac{2}{m}\right] \) 时, \( f'(x) \leq 0 \), 当 \( x \in \left(\frac{2}{m}, 2\right) \) 时, \( f'(x) > 0 \quad \quad \quad \quad \quad \quad \quad \quad \ \ \ (4) \)

即 \( f(x) \) 的单调增区间为 \(\left(-\infty, \frac{2}{m}\right] \), 单调减区间为 \(\left[\frac{2}{m}, 2\right) \quad \quad \quad \quad \quad \quad \quad \quad \quad (5) \)

(2) 由 (1) 知, 当 \( m > 0, \quad x \in [1, 2] \) 时, \( f'(x) > 0 \) 恒成立. \quad \quad \quad \quad \quad \quad \quad \quad \quad (6)
```