```markdown
19. 解: (1) 取 \(EF\) 的中点 \(G\)，连接 \(DG, CG\)

- \( \because \) 四边形 \(ADEF, F_1\) 和 \(BCEF_2\) 都是菱形, 
  \(\angle DEF_1 = \angle CEF_2 = 60^\circ\)

\( \therefore \)
\[ DG \perp EF \]
\[ \boxed{BC = 2} \]
\[ DG = CG = \sqrt{3} \]
\[ \boxed{CD = AB = \sqrt{6}} \]

即有
\[ DG^2 + CG^2 = CD^2, \quad DG \perp CG \]
\[ \boxed{CG \parallel EF = G, \quad CG, \quad EF \subset \text{平面} BCEF} \]

\[ \because \]
\[ DG \perp \text{平面} BCEF \]
\[ \therefore \]
\[ \because DG \perp \text{平面} AFED \]

- 平面 \(AFED \perp \text{平面} BCEF\) 
- (2) 连接 \(DF, DB\)

由 (1) 知
\[ DG \perp \text{平面} BCEF, \quad \text{同理 } CG \perp \text{平面} AFED \]

\[ H_5^{\triangle BDFCEF} = 2 \sqrt{3} = 2 \frac{1}{2} \times 2 \sqrt{3} = \sqrt{3} \]

\[ V = V_{D-BCEF} + V_{D-ABF} - V_{D-AFDF} + V_{D-BAF} = \frac{1}{3}
S_{\triangle BDFCEF} \cdot DG + \frac{1}{3} S_{\triangle ADF} \cdot CG \]

- \(\frac{1}{3} \times \sqrt{3} \times \sqrt{3} + \frac{1}{3} \times \sqrt{3} \times \sqrt{3}\)

\[ = 3 \]

20. 解: (1) \( f'(x) = \frac{-mx^2 + 2(m-1)x + 4}{e^t} = \frac{-(mx+2)(x-2)}{e^t} \quad (m>0) \]

令 \( x = f(x) \), 解得
\[ x = \frac{-2}{m}, \quad x = 2 \]
当 \( x \in (-\infty, -\frac{2}{m}]\), \( f(x) < 0 \),
当 \( x \in (-\frac{2}{m}, e ] \), \( f'(x) > 0 \),

当 \( x \in [2, +\infty) \), \( f'(x) \leq 0 \)

即 \( f(x) \) 的单调区间为 \((- \frac{2}{m}, e), \text{增减区间为}(-\infty, -\frac{2}{m}], [2, +\infty) \)

- (2) 由 (1) 知, 当 \( m > 0, x \in [0, 2] \subset [1, 2] \), \( f'(x) \geq 0 \) 恒成立.

\[ \therefore f(x) \text{ 在 } [1, 2] \text{ 上为增函数.} \]

即
\[ f(x)_{\max} = f(2) = \frac{4m + 2}{e^t}, \quad f(x)_{\min} = f(1) = \frac{m}{e} \]

\( f(x)_\max - f(x)_\min = g(m) = f(x)_\max - f(x)_\min = \frac{(4-e)m+2}{e^t} \)

即
\[ m \leq \frac{2}{4-e} \]

\( x_m > 0 \)
\[ \therefore m \in \left(0, \frac{2}{4-e}\right] \]

故 \( m \) 的取值范围
\[ \boxed{\left(0, \frac{2}{4-e}\right]} \]


21. 解: (1) \( \cdot e = \frac{c}{a} = \frac{\sqrt{2}}{2}, \quad \cdot c^2 = \frac{1}{2} a^2, \)
\(\cdot b^2 = a^2 - c^2 = \frac{1}{2} a^2 \)

- 椭圆的中心 \( O \) 到直线 \(x+y-2b=0\) 的距离为
  \(\sqrt{5}/2, \quad \cdot \frac{-2b}{\sqrt{2}} = 5\sqrt{2}, \quad \cdot b = 5. . .; \ b^2 = 25, \quad a^2 = 2b^2 = 50.\)

- 插图 \(C\) 的方程为
  \[ \frac{x^2}{50} + \frac{y^2}{25} = 1 \]

(2) 由 (1) 可知 \( F(5, 0) \), 由题可知直线 \(AB\) 的方程为 
\[ y = \frac{\sqrt{2}(x-5)} \]

与椭圆 \(C\) 的方程联立:
\[ \frac{x^2}{50} + \frac{y^2}{25} = 1 \]

消去得到
\[ x^2 - 8x + 10 = 0 \]

设 \(A(x_1, y_1)\), \(B(x_2, y_2)\), 则有 
\[ x_1 + x_2 = 8, \quad x_1 x_2 = 10 \]

设 \( (x, y) \), 且 \( \vec{OQ} = \lambda \vec{OA} + \mu \vec{OB} \) 得
\[ (x, y) = \lambda (x_1, y_1) + \mu (x_2, y_2) = (\lambda x_1 + \mu x_2, \lambda y_1 + \mu y_2) \]

\[
\left\{
\begin{aligned}
  & x = \lambda x_1 + \mu x_2, \\
  & y = \lambda y_1 + \mu y_2.
\end{aligned}
\right.
\]
```
